only use the RepPredicate typeclass for create_predicate,
but no generic rep appearing in sepclauses, because that would
have to be used very pervasively in all lemmas, so array lemmmas
would all be stated in terms of rep instead of array, and unfolding/
folding rep also is a bit more complicated

bedrock2/src/bedrock2Examples/LiveVerif/ZSemantics.v
@@ -176,6 +176,9 @@ Definition array_t(tp: Type)(nElems: Z) := list tp.
 
 Global Hint Opaque uint_t array_t : typeclass_instances.
 
+Definition RepPredicate(T: Type) := T -> Z -> mem -> Prop.
+Existing Class RepPredicate.
+
 Section WithParams.
   Context {width: Z}.
 
@@ -244,7 +247,7 @@ Section WithParams.
       | cons h tl => sep (elem h start) (rec tl (start + elemSize))
       end.
 
-  Definition array{T: Type}(elem: T -> Z -> mem -> Prop)(n: Z){elemSize: Z}
+  Definition array{T: Type}(elem: RepPredicate T)(n: Z){elemSize: Z}
     {H: forall v, PredicateSize (elem v) elemSize}(vs: list T)(addr: Z): mem -> Prop :=
     sep (emp (len vs = n)) (array_rec elem elemSize vs addr).
 
@@ -2069,17 +2072,18 @@ Section WithNonmaximallyInsertedA.
   Proof. intros. reflexivity. Qed.
 End WithNonmaximallyInsertedA.
 
-Class RepPredicate(T: Type) := rep: T -> Z -> mem -> Prop.
-
 (* ARP responder example *)
 
 Definition MAC := array_t (uint_t 8) 6.
+Global Hint Extern 1 (RepPredicate MAC) => exact (array (uint 8) 6) : typeclass_instances.
+
 Definition IPv4 := array_t (uint_t 8) 4.
+Global Hint Extern 1 (RepPredicate IPv4) => exact (array (uint 8) 4) : typeclass_instances.
 
 Definition ARPOperationRequest: Z := 1.
 Definition ARPOperationReply: Z := 2.
 
-Record ARPPacket := mkARPPacket {
+Record ARPPacket_t := mkARPPacket {
   htype: uint_t 16; (* hardware type *)
   ptype: uint_t 16; (* protocol type *)
   hlen: uint_t 8;   (* hardware address length (6 for MAC addresses) *)
@@ -2091,7 +2095,7 @@ Record ARPPacket := mkARPPacket {
   tpa: IPv4; (* target protocol address *)
 }.
 
-Record EthernetHeader := mkEthernetHeader {
+Record EthernetHeader_t := mkEthernetHeader {
   dstMAC: MAC;
   srcMAC: MAC;
   etherType: uint_t 16;
@@ -2101,23 +2105,27 @@ Record EthernetHeader := mkEthernetHeader {
 Global Instance Bool_eqb_spec: EqDecider Bool.eqb.
 Proof. intros. destruct x; destruct y; constructor; congruence. Qed.
 
-Global Instance uint_t_predicate(nbits: Z): RepPredicate (uint_t nbits) := uint nbits.
+Global Hint Extern 1 (RepPredicate (uint_t ?nbits)) =>
+  exact (uint nbits) : typeclass_instances.
 
-Global Instance array_t_predicate(T: Type)(n: Z)(elem_pred: RepPredicate T)(elemSize: Z)
-  (Hsz: forall v : T, PredicateSize (rep v) elemSize): RepPredicate (array_t T n) :=
-  array (@rep T elem_pred) n.
+Global Hint Extern 1 (RepPredicate (array_t ?T ?n)) =>
+ exact (@array T _ n _ _) : typeclass_instances.
 
 Ltac create_predicate_rec refine_already_introd :=
   lazymatch goal with
-  | |- forall (lastField: _), Z -> ?mem -> Prop =>
+  | |- forall (lastField: ?T), Z -> ?mem -> Prop =>
       let f := fresh lastField in
       intro f;
       refine_already_introd;
-      exact (rep f)
-  | |- forall (name: _), _ =>
+      match constr:(_ : RepPredicate T) with
+      | ?p => exact (p f)
+      end
+  | |- forall (name: ?T), _ =>
       let f := fresh name in
       intro f;
-      create_predicate_rec ltac:(refine_already_introd; refine (sepapp (rep f) _))
+      match constr:(_ : RepPredicate T) with
+      | ?p => create_predicate_rec ltac:(refine_already_introd; refine (sepapp (p f) _))
+      end
   end.
 
 Ltac create_predicate :=
@@ -2128,10 +2136,10 @@ Ltac create_predicate :=
              exact t'
   end.
 
-Global Instance ARPPacket_predicate: RepPredicate ARPPacket :=
+Global Instance ARPPacket: RepPredicate ARPPacket_t :=
   ltac:(create_predicate).
 
-Global Instance EthernetHeader_predicate: RepPredicate EthernetHeader :=
+Global Instance EthernetHeader: RepPredicate EthernetHeader_t :=
   ltac:(create_predicate).
 
 (* New Feature TODO:
@@ -2235,24 +2243,17 @@ Ltac purify :=
 Inductive unfold_step{V: Type}(addr: Z)(pred: V -> Z -> mem -> Prop): Prop :=
   mk_unfold_step.
 
-Ltac unfold_until_sepapp t :=
-  lazymatch t with
-  | (sepapp _ _) _ => t
-  | _ => let h := head t in
-         let u := eval cbv beta iota delta[h] in t in
-         unfold_until_sepapp u
-  end.
-
 Ltac unfold_pred a pred :=
   let name := fresh "step0" in
   pose proof (mk_unfold_step a pred) as name;
+  let h := head pred in
   repeat match goal with
     | H: context C[pred ?v a] |- _ =>
-        let u := unfold_until_sepapp (pred v a) in
+        let u := eval unfold h in (pred v a) in
         let t := context C[u] in
         change t in H
     | |- context C[pred ?v a] =>
-        let u := unfold_until_sepapp (pred v a) in
+        let u := eval unfold h in (pred v a) in
         let t := context C[u] in
         change t
     end.
@@ -2270,17 +2271,17 @@ Ltac fold_pred :=
   end.
 
 (* not a Lemma because this kind of goal will be solved inline by sepcalls canceler *)
-Goal forall (bs: list (uint_t 8)) (R: mem -> Prop) a m (Rest: EthernetHeader -> Prop),
+Goal forall (bs: list (uint_t 8)) (R: mem -> Prop) a m (Rest: EthernetHeader_t -> Prop),
     sep (array (uint 8) 14 bs a) R m ->
-    exists h, sep (rep h a) R m /\ Rest h.
+    exists h, sep (EthernetHeader h a) R m /\ Rest h.
 Proof.
   intros.
   purify.
   eexists (mkEthernetHeader _ _ _).
 
   match goal with
-  | |- context[rep ?h ?a] =>
-      pose proof (_ : PredicateSize (rep h) _) as Hsz
+  | |- context[EthernetHeader ?h ?a] =>
+      pose proof (_ : PredicateSize (EthernetHeader h) _) as Hsz
   end.
   cbn in Hsz. (* --> clause in goal has same size as clause in hyp H *)
   clear Hsz.
@@ -2295,11 +2296,6 @@ Proof.
    *)
 
   match goal with
-  | |- context[@rep ?T ?pred ?h ?a] =>
-      let r := unfold_until_sepapp (@rep T pred h a) in idtac r
-  end.
-
-  match goal with
   | |- context[?folded ?v a] => unfold_pred a folded
   end.
 
@@ -2310,17 +2306,15 @@ Proof.
   2: {
     repeat rewrite List.len_from; lia.
   }
-  rewrite <- sepapp_assoc in H.
 
   (* TODO if "rep ?dstMAC" was a nested record as well that needs to be unfolded,
      how would we record it, given that we have no address?
-  unfold rep.
+     --> don't record address, only the predicate *)
   split. 1: exact H. (* instantiates all evars *)
 
   fold_pred.
 
-  unfold_pred a EthernetHeader_rep.
-  *)
+  unfold_pred a EthernetHeader.
 
 Abort.
 
